Fix translation from L3 to simple_cps expressions, erasing Product, Inductive and Sort types.
- We are missing information when translating case expressions,
  to give in each branch the number of constructor arguments.
  The inductive type is no longer available in L3, so this should
  be kept around.

- The translation of Fix is tricky as it changes the local variables
  during the translation, with some shifting involved to go over a 
  tuple binder. WIP.

Nonetheless, 0%nat can be translated down to greg's cps and evaluated
correctly.

theories/L4_CPS/L3_to_L4.v
@@ -1,4 +1,3 @@
-
 (** Naive conversion to continuation-passing style for a core language including
     mutually recursive functions, data constructors, and pattern matching.
 *)
@@ -12,48 +11,203 @@ Require Import L3.program.
 
 Require L3.
 Module L3eval := L3.wndEval.
-Module L3 := L3.term.
-Require Import  simpleCPS.
+Module L3t := L3.term.
+Module L3U := L3.unaryApplications.
+Require Import simple_cps.
 
 Definition dcon_of_con (i : inductive) (n : nat) := N.of_nat n.
 
-Fixpoint translate (t : L3.Term) : simpleCPS.exp :=
-  match t with
-  | L3.TRel n => Var_e (N.of_nat n)
-  | L3.TSort s => Var_e 0 (* encode with TConst ? *)
-  | L3.TProd n t => Var_e 0  (* same ? *)
-  | L3.TLambda n t => Lam_e (translate t)
-  | L3.TLetIn n t u => Let_e (translate t) (translate u)
-  | L3.TApp t u => App_e (translate t) (translate u)
-  | L3.TConst s => Var_e 0 (* FIXME *)
-  | L3.TInd i => Var_e 0 (* FIXME *)
-  | L3.TConstruct ind c args =>
-    let fix args' l :=
-        match l with
-        | L3.tnil => nil
-        | L3.tcons t ts => cons (translate t) (args' ts)
-        end
-    in Con_e (dcon_of_con ind c) (args' args)
-  | L3.TCase n t brs =>
-    let fix brs' n l :=
-      match l with
-      | L3.tnil => nil
-      | L3.tcons t ts => cons (n, 0 (* FIXME *), translate t) (brs' (n + 1)%N ts)
-      end
-    in Match_e (translate t) (brs' (0%N) brs)
-  | L3.TFix d n =>
-    let fix defs' l :=
-        match l with
-        | L3.dnil => nil
-        | L3.dcons na t k l' => cons (translate t) (defs' l')
-        end
-    in Proj_e (Fix_e (defs' d)) (N.of_nat n)
+(** Unit type single constructor *)
+Definition dummy := Con_e 0 [].
+
+(** Definition environment *)
+Definition env := list (string * exp).
+
+Fixpoint cst_offset (e : env) (s : string) : N :=
+  match e with
+  | [] => 0%N
+  | (c, e) :: tl => if string_eq_bool s c then 0 else cst_offset tl s + 1
   end.
 
-Theorem translate_correct (e : environ) (t t' : L3.Term) :
+(** Inductive environment: disappears at this stage *)
+Definition ienv := list (string * itypPack).
+
+Section TermTranslation.
+  Variable ie : ienv.
+  Variable e : env.
+
+  (* Fixpoint fix_subst (n : nat) := *)
+  (*   match n with *)
+  (*   | 0%nat => [Proj_e (Var_e 0%N) 0%N] *)
+  (*   | S n' => *)
+  (*     (Proj_e (Var_e 0%N) (N.of_nat n)) :: fix_subst n' *)
+  (*   end. *)
+
+  Fixpoint fix_subst (n : nat) (k : N) (t : exp) :=
+    match n with
+    | 0%nat => (* Go over the tuple binder *) shift 1 k t
+    | S n' =>
+      Let_e (Proj_e (Var_e k) (N.of_nat n')) (fix_subst n' (k + 1) t) 
+    end.
+  
+  Fixpoint translate (k : N) (t : L3t.Term) : exp :=
+    match t with
+    | L3t.TRel n => Var_e (N.of_nat n)
+    | L3t.TSort s => (* Erase *) dummy
+    | L3t.TProd n t => (* Erase *) dummy
+    | L3t.TLambda n t => Lam_e (translate (k+1) t)
+    | L3t.TLetIn n t u => Let_e (translate k t) (translate (k+1) u)
+    | L3t.TApp t u => App_e (translate k t) (translate k u)
+    | L3t.TConst s => (* Transform to let-binding *)
+      Var_e (cst_offset e s + k)
+    | L3t.TInd i => (* Erase *) dummy
+    | L3t.TConstruct ind c args =>
+      let fix args' l :=
+        match l with
+        | L3t.tnil => nil
+        | L3t.tcons t ts => cons (translate k t) (args' ts)
+        end
+      in Con_e (dcon_of_con ind c) (args' args)
+    | L3t.TCase n t brs =>
+      let fix brs' n l :=
+          match l with
+          | L3t.tnil => nil
+          | L3t.tcons t ts =>
+            cons (n, 0 (* Number of args of n, impossible to infer here *),
+                  translate k t) (brs' (n + 1)%N ts)
+          end
+      in Match_e (translate k t) (brs' (0%N) brs)
+    | L3t.TFix d n =>
+      let len := L3t.dlength d in
+      let subst := fix_subst len 0 in
+      let fix defs' l :=
+          match l with
+          | L3t.dnil => nil
+          | L3t.dcons na t _ l' =>
+            let t' := translate (k + N.of_nat len) t in
+              cons (subst t') (defs' l')
+          end
+      in      
+      Proj_e (Fix_e (defs' d)) (N.of_nat n)
+    end.
+
+  (** The [TFix d n] block assumes that recursive calls to [di] in [d] are of the 
+      form [TRel ki], while in the cps exp encoding, this becomes a projection
+      of a tuple, we hence have to substitute these rels in [t] by the right
+      projections. Actually, we have no substitution operation on L3 terms, so
+      we have to use let-bindings instead. *)
+  
+End TermTranslation.
+
+Definition translate_env (e : environ) : env :=
+  fold_right
+    (fun x acc => match x with
+               | (s, ecTrm t) =>
+                 let t' := translate acc 0%N t in
+                   (s, t') :: acc
+               | (s, ecTyp _) => acc
+               end) [] e.
+
+Definition mkLets (e : env) (t : exp) :=
+  fold_left (fun acc (x : string * exp) => let (s, t) := x in Let_e t acc) e t.
+
+Definition translate_program (e : environ) (t : L3t.Term) : exp :=
+  let e' := translate_env e in
+    mkLets e' (translate e' 0 t).
+              
+Theorem translate_correct (e : environ) (t t' : L3t.Term) :
   L3eval.wndEval e t t' -> (* small step non-deterministic *)
-  eval (translate t) (translate t') (* big-step deterministic *).
+  eval (translate_program e t) (translate_program e t') (* big-step deterministic *).
 Proof.
-  induction 1. simpl. red in H. 
+  induction 1. simpl. red in H.
+Admitted.
 
+(** start-to-L4 translations **)
 
+Definition myprogram_Program (pgm : program) :=
+  do pgm0 <- malecha_L1.program_Program pgm (Ret nil);
+    let e' := stripEvalCommute.stripEnv (program.env pgm0) in
+    match L3U.stripEnv e' with
+    | Some senv => 
+      match L3U.strip e' (stripEvalCommute.strip (program.main pgm0)) with
+      | Some smain => Ret {| main := smain; L3.program.env := senv |}
+      | None => Exc "Error in stripping"
+      end
+    | None => Exc "Error while stripping environment"
+    end.
+
+Definition program_exp (pgm:program) : exception exp :=
+  do prg <- myprogram_Program pgm;
+      let (main, env) := prg in
+      Ret (translate_program env main).
+
+Definition term_exp (e:program.environ) (t:term) : exception exp :=
+  let e' := stripEvalCommute.stripEnv e in
+  match L3U.term_Term e' t with
+  | None => Exc "Error while translating term to L3"
+  | Some trm =>
+    match L3U.stripEnv e' with
+    | None => Exc "Error while stripping environment"
+    | Some e => Ret (translate_program e trm)
+    end
+  end.
+
+(** Testing the compiler *)
+
+Require Import Template.Template.
+Definition Nat := nat.
+Definition typedef := ((fun (A:Type) (a:A) => a) Nat 1%nat).
+
+Quote Definition q_typedef := Eval compute in typedef.
+Quote Recursively Definition p_typedef := typedef.
+Definition L1_typedef :=
+  Eval compute in malecha_L1.program_Program p_typedef (Ret nil).
+
+Definition P_typedef := Eval compute in program_exp p_typedef.
+
+Fixpoint slowFib (n:nat) : nat :=
+  match n with
+    | 0%nat => 0
+    | S m => match m with
+               | 0%nat => 1
+               | S p => slowFib p + slowFib m
+             end
+  end.
+Eval compute in (slowFib 0).
+Eval compute in (slowFib 1).
+Eval compute in (slowFib 2).
+Eval compute in (slowFib 3).
+Eval compute in (slowFib 4).
+
+Fixpoint idn (n : nat) : nat :=
+  match n with 0%nat => 0 | S n => S (idn n) end.
+
+Quote Recursively Definition p_0 := 0.
+Quote Recursively Definition p_idn := idn.
+Quote Recursively Definition p_idn1 := (idn 1).
+
+Quote Recursively Definition p_slowFib1 := (slowFib 1).
+
+Quote Recursively Definition p_add := Nat.add.
+Quote Recursively Definition p_add01 := (Nat.add 0%nat 1).
+Transparent N.add.
+Eval compute in program_exp p_add.
+
+Definition compile (p : program) : exception cps :=
+  do e <- program_exp p; Ret (cps_cvt_prog e).
+
+Definition paddexp := Eval compute in compile p_add.
+
+Definition padd01 := Eval compute in compile p_add01.
+
+Definition run (p : program) : exception ans :=
+  do c <- compile p; Ret (eval_c_n 1000 c).
+Eval compute in run p_0.
+
+Eval compute in program_exp p_add01.
+Eval compute in run p_add01.
+
+Eval compute in program_exp p_idn.
+
+Eval compute in program_exp p_idn1.
+Eval compute in run p_idn1.
